crypto/bignum/Hacl.Spec.Bignum.Fmul.fst
@@ -193,3 +193,29 @@ let rec mul_shift_reduce_spec input input2 =
 
 let fmul_pre (input:seqelem) (input2:seqelem) : GTot Type0 =
   mul_shift_reduce_pre (Seq.create len wide_zero) input input input2 len
+  /\ carry_wide_pre (mul_shift_reduce_spec input input2) 0
+  /\ carry_top_wide_pre (carry_wide_spec (mul_shift_reduce_spec input input2) 0)
+  /\ copy_from_wide_pre (carry_top_wide_spec (carry_wide_spec (mul_shift_reduce_spec input input2) 0))
+  /\ carry_0_to_1_pre (copy_from_wide_spec (carry_top_wide_spec (carry_wide_spec (mul_shift_reduce_spec input input2) 0)))
+
+#set-options "--initial_fuel 0 --max_fuel 0"
+
+val fmul_spec:
+  input:seqelem -> input2:seqelem{fmul_pre input input2} ->
+  Tot (output:seqelem{seval output % prime = (seval input * seval input2) % prime})
+let fmul_spec input input2 =
+  let tmp = Seq.create len wide_zero in
+  let output1 = mul_shift_reduce_spec input input2 in
+  let output2 = carry_wide_spec output1 0 in
+  lemma_carry_top_wide_spec output2;
+  let output3 = carry_top_wide_spec output2 in
+  lemma_copy_from_wide output3;
+  let output4 = copy_from_wide_spec output3 in
+  carry_0_to_1_spec output4
+
+#set-options "--z3rlimit 40"
+
+
+val lemma_whole_slice: #a:Type -> s:Seq.seq a -> Lemma
+  (Seq.slice s 0 (Seq.length s) == s)
+let lemma_whole_slice #a s = Seq.lemma_eq_intro (Seq.slice s 0 (Seq.length s)) s
